theories/case_studies/eio/atomics.v
@@ -1,0 +1,52 @@
+From program_logic Require Import reasoning_rules.
+
+Definition sub_redexes_are_values (e : expr) :=
+  ∀ K e', e = fill K e' → to_val e' = None → K = [].
+
+Definition head_atomic (a : atomicity) (e : expr) : Prop :=
+  ∀ σ e' σ' ,
+    head_step e σ e' σ' →
+    if a is WeaklyAtomic then irreducible e' σ' else is_Some (to_val e').
+
+Lemma ectx_language_atomic a e :
+  head_atomic a e → sub_redexes_are_values e → Atomic a e.
+Proof.
+  intros Hatomic_step Hatomic_fill σ e' κ σ' efs H.
+  unfold language.prim_step in H. simpl in H. unfold prim_step' in H.
+  destruct κ, efs; try by destruct H.
+  destruct H as [K e1' e2' -> -> Hstep].
+  assert (K = []) as -> by eauto 10 using val_head_stuck.
+  simpl fill. simpl fill in Hatomic_step.
+  eapply Hatomic_step. by apply Hstep.
+Qed.
+
+Lemma fill_val2 (k : ectx) (e: expr) :
+  is_Some (to_val (fill k e)) → is_Some (to_val e).
+Proof.
+  intros (v & [-> ->]%fill_val).
+  simpl. done.
+Qed.
+
+Lemma fill_no_value (k: ectx) (e: expr) (v: val) :
+  to_val e = None → fill k e = v → False.
+Proof.
+  intros Hv Hfill.
+  specialize (fill_not_val k _ Hv) as Hfill'.
+  rewrite Hfill in Hfill'.
+  simpl in Hfill'. discriminate Hfill'.
+Qed.
+
+Local Ltac solve_atomic := 
+  apply ectx_language_atomic;
+  [ inversion 1; naive_solver
+  | intros [|f?] ? H ?; [|
+    exfalso; destruct f; inversion H; by eapply fill_no_value ]].
+
+Global Instance store_atomic v1 v2 : Atomic StronglyAtomic (Store (Val v1) (Val v2)).
+Proof. by solve_atomic. Qed.
+
+Global Instance load_atomic v : Atomic StronglyAtomic (Load (Val v)).
+Proof. by solve_atomic. Qed.
+
+Global Instance alloc_atomic v : Atomic StronglyAtomic (Alloc (Val v)).
+Proof. by solve_atomic. Qed.
