theories/case_studies/eio/concurrent_queue.v
@@ -1,0 +1,56 @@
+From iris.base_logic.lib Require Import iprop.
+From program_logic Require Import reasoning_rules.
+
+Section concurrent_queue.
+Context `{!heapGS Σ}.
+
+Parameter queue_create : val.
+Parameter queue_push   : val.
+Parameter queue_pop    : val.
+
+Parameter is_queue :
+  val -d> (val -d> iPropO Σ) -d> iPropO Σ.
+  
+Parameter is_queue_ne_proof : ∀ (q: val) (n: nat),
+  Proper ((dist n) ==> (dist n)) (is_queue q).
+
+Parameter is_queue_proper_proof : ∀ (q: val),
+  Proper ((≡) ==> (≡)) (is_queue q).
+
+Parameter is_queue_Persistent_proof : ∀ (q: val) (I: val -> iProp Σ),
+  Persistent (is_queue q I).
+
+Parameter queue_create_spec : ∀ (Ψ1 Ψ2: iEff Σ),
+  ⊢ EWP queue_create #() <| Ψ1 |> {| Ψ2 |} {{ q,
+      ∀ I, is_queue q I }}.
+
+Parameter queue_push_spec : ∀ (Ψ1 Ψ2: iEff Σ) (q: val) (I: val -> iProp Σ) v,
+  is_queue q I -∗
+    I v -∗
+      EWP queue_push q v <| Ψ1 |> {| Ψ2 |} {{ _, True }}.
+
+Parameter queue_pop_spec : ∀ (Ψ1 Ψ2: iEff Σ) (q: val) (I: val -> iProp Σ),
+  is_queue q I -∗
+    EWP queue_pop q <| Ψ1 |> {| Ψ2 |} {{ y,
+      ⌜ y = NONEV ⌝ ∨ 
+      ∃ (v: val), ⌜ y = SOMEV v ⌝ ∗ I v }}.
+
+Global Instance is_queue_ne q n:
+  Proper ((dist n) ==> (dist n)) (is_queue q).
+Proof.
+  apply is_queue_ne_proof.
+Qed.
+
+Global Instance is_queue_proper q :
+  Proper ((≡) ==> (≡)) (is_queue q).
+Proof.
+  apply is_queue_proper_proof.
+Qed.
+
+Global Instance is_queue_Persistent q I:
+  Persistent (is_queue q I).
+Proof.
+  apply is_queue_Persistent_proof.
+Qed.
+
+End concurrent_queue.
