theories/case_studies/eio/cqs.v
@@ -1,0 +1,104 @@
+From iris.proofmode Require Import base tactics classes.
+From iris.algebra Require Import excl_auth gset gmap agree csum frac excl.
+From iris.base_logic Require Import invariants.
+From iris.base_logic.lib Require Import iprop wsat saved_prop.
+From program_logic Require Import reasoning_rules.
+From case_studies Require Import list_lib .
+
+(* An axiomatization of CQS *)
+Section cqs.
+Context `{!heapGS Σ, !ListLib Σ}.
+
+Variable R : iProp Σ.
+
+Definition is_waker (P: val -> iProp Σ) (k : val): iProp Σ := ∀ v, P v -∗ EWP (k v) {{_, True}}.
+Definition V' v := (⌜ v = #() ⌝ ∗ R)%I.
+
+Parameter cqs_new     : val.
+Parameter cqs_suspend    : val.
+Parameter cqs_resume_all : val.
+Parameter cqs_try_cancel     : val.
+
+(* put the suspend proposition into the queue *)
+Parameter is_thread_queue :
+  val -> iProp Σ.
+Parameter thread_queue_state :
+  nat -> iProp Σ.
+Parameter resume_all_permit :
+  iProp Σ.
+Parameter is_thread_queue_suspend_result :
+  gname -> val -> val -> iProp Σ.
+Parameter suspension_permit :
+  iProp Σ.
+
+Parameter is_thread_queue_Persistent_proof : ∀ q,
+  Persistent (is_thread_queue q).
+Parameter thread_queue_state_timeless_proof : ∀ n,
+  Timeless (thread_queue_state n).
+Parameter resume_all_permit_timeless_proof : 
+  Timeless (resume_all_permit).
+
+Parameter thread_queue_append': ∀ n q E',
+  is_thread_queue q -∗
+  ▷ thread_queue_state n ={E'}=∗
+  thread_queue_state (S n) ∗ suspension_permit .
+    
+Parameter newThreadQueue_spec:
+  ⊢ EWP cqs_new #()
+  {{ q, is_thread_queue q 
+      ∗ thread_queue_state 0 ∗ resume_all_permit }}.
+        
+(* todo use parameters correctly and make V'/R also a parameter. *)
+Parameter cqs_suspend_spec: ∀ q k ,
+      is_thread_queue q ∗ 
+  (* a generic permit to call suspend *)
+      suspension_permit ∗ 
+  (* the WP of the closure k so that we can create a callback. *)
+      is_waker V' k
+  ⊢
+    EWP cqs_suspend q k
+  {{ v, ⌜v = NONEV⌝ ∨
+                ∃ γk v', ⌜v = SOMEV v'⌝ ∗
+                         is_thread_queue_suspend_result γk v' k }}.
+
+Parameter cqs_try_cancel_spec: ∀ q γk r k,
+  (* the invariant about the state of CQS. *)
+      is_thread_queue q ∗ 
+      is_thread_queue_suspend_result γk r k
+  ⊢
+    EWP cqs_try_cancel r
+  {{ v, ∃ (b: bool), ⌜ v = #b ⌝ ∗ if b then 
+                  (* is_waker gives us the WP for executing k *)
+                  is_waker V' k 
+                  (* if cancellation fails we don't know anything (on the metalevel we know that another thread will eventually call k, but we don't have this linearity in the Iris proof yet). *)
+                  else True }}.
+
+Parameter cqs_resume_all_spec: ∀ q n,
+    is_thread_queue q ∗
+    □ ▷ R ∗
+    resume_all_permit ∗
+    thread_queue_state n
+  ⊢
+    EWP cqs_resume_all q
+    {{ _, True }}.
+
+Global Instance is_cqs_Persistent q:
+  Persistent (is_thread_queue q).
+Proof.
+  apply is_thread_queue_Persistent_proof.
+Qed.
+
+Global Instance thread_queue_state_Timeless n:
+  Timeless (thread_queue_state n).
+Proof.
+  apply thread_queue_state_timeless_proof.
+Qed.
+
+Global Instance resume_all_permit_Timeless:
+  Timeless (resume_all_permit).
+Proof.
+  apply resume_all_permit_timeless_proof.
+Qed.
+
+End cqs.
+
